101

HumanEvalLean/HumanEval101.lean
@@ -1,5 +1,108 @@
-def words_string : Unit :=
-  ()
+module
+
+import Std
+open Std Std.Do
+
+set_option mvcgen.warning false
+
+def delimiters : TreeSet Char := .ofList [' ', ',', '\t', '\n', '\r']
+
+def wordsString (str : String) : Array String :=
+  str.split (· ∈ delimiters)
+    |>.filter (! ·.isEmpty)
+    |>.map String.Slice.toString
+    |>.toArray
+
+def wordsString₂ (str : String) : Array String := Id.run do
+  let mut words : Array String := #[]
+  let mut currentWord : String := ""
+  for c in str.chars do
+    if c ∈ delimiters then
+      if ! currentWord.isEmpty then
+        words := words.push currentWord
+        currentWord := ""
+    else
+      currentWord := currentWord.push c
+  if ! currentWord.isEmpty then
+    words := words.push currentWord
+  return words
+
+/-!
+## Tests
+-/
+
+example : wordsString "Hi, my name is John" = #["Hi", "my", "name", "is", "John"] := by
+  native_decide
+
+example : wordsString "One, two, three, four, five, six" =
+      #["One", "two", "three", "four", "five", "six"] := by
+  native_decide
+
+example : wordsString "Hi, my name" = #["Hi", "my", "name"] := by
+  native_decide
+
+example : wordsString "One,, two, three, four, five, six," =
+      #["One", "two", "three", "four", "five", "six"] := by
+  native_decide
+
+example : wordsString "ahmed     , gamal" = #["ahmed", "gamal"] := by
+  native_decide
+
+example : wordsString "" = #[] := by
+  native_decide
+
+/-!
+# Verification
+-/
+
+@[grind =]
+theorem not_contains_empty {c : Char} :
+    "".contains c = false := by
+  sorry
+
+@[grind =]
+theorem contains_push {s : String} {c d : Char} :
+    (s.push c).contains d = (s.contains d || c = d) := by
+  sorry
+
+theorem not_contains_of_mem_delimiters {s : String} {c : Char} (h : c ∈ delimiters) :
+    (wordsString₂ s).all (! ·.contains c) := by
+  generalize hret : wordsString₂ s = ret
+  apply Id.of_wp_run_eq hret
+  mvcgen
+  case inv1 => exact ⇓⟨_, currentWord, words⟩ => ⌜¬ currentWord.contains c ∧ words.all (! ·.contains c)⌝
+  all_goals grind
+
+@[simp, grind =]
+theorem toList_chars_empty : "".chars.toList = [] := by
+  sorry
+
+@[simp, grind =]
+theorem isEmpty_empty : "".isEmpty := by
+  sorry
+
+@[simp, grind =]
+theorem wordsString₂_empty :
+    wordsString₂ "" = #[] := by
+  simp [wordsString₂, ← Iter.forIn_toList]
+
+theorem wordsString₂_push_of_mem {s : String} {c : Char} (h : c ∈ delimiters) :
+    wordsString₂ (str.push c) = wordsString₂ str := by
+  sorry
+
+theorem wordsString₂_push {s : String} {c : Char} :
+    wordsString₂ (str.push c) =
+      if c ∈ delimiters then
+        wordsString₂ str
+      else if str.startPos.get?.all (· ∈ delimiters) then
+        (wordsString₂ str).push (Char.toString c)
+      else
+        (wordsString₂ str).modify ((wordsString₂ str).size - 1) (·.push c) := by
+  sorry
+
+theorem wordsString_eq_append {s t : String} {c : Char} (h : c ∈ delimiters) :
+    wordsString₂ (s ++ Char.toString c ++ t) = wordsString₂ s ++ wordsString₂ t := by
+  sorry
 
 /-!
 ## Prompt
@@ -10,7 +113,7 @@ def words_string(s):
     """
     You will be given a string of words separated by commas or spaces. Your task is
     to split the string into words and return an array of the words.
-    
+
     For example:
     words_string("Hi, my name is John") == ["Hi", "my", "name", "is", "John"]
     words_string("One, two, three, four, five, six") == ["One", "two", "three", "four", "five", "six"]
